\begin{proof}
Let $M = (Q, \Sigma, \delta, q_0, F)$ be an $\epsilon$-NFA.
Construct a DFA $M' = (2^Q, \Sigma, \delta', q'_0, F')$ by putting
\[
q'_0 = \overline{\{q_0\}}, \quad F' = \{P \subset Q \mid P \cap F \ne \emptyset\},
\]
and defining the transition function by
\[
\delta'(P, a) = \overline{\delta(P, a)}.
%= \overline{\bigcup_{p \in P} \delta(p, a)}.
\]
We claim that for any word $w \in \Sigma^*$ holds
\begin{equation}
\label{eqn:DeltaD=DeltaE}
\widehat{\delta'}(q'_0, w) = \widehat{\delta}(q_0, w),
\end{equation}
where $\widehat{\delta}$ and $\widehat{\delta'}$ are the extended transition functions of $M$ and $M'$.
This is proved by induction on the length of the word $w$.
The base: $|w| = 0$, that is $w = \epsilon$. We have
\[
\widehat{\delta'}(q'_0, \epsilon) = q'_0 = \overline{\{q_0\}} = \widehat{\delta}(q_0, \epsilon).
\]
The induction step: assume \eqref{eqn:DeltaD=DeltaE} holds for all words of length $n$.
Any word of length $n+1$ has the form $wa$, where $|w| = n$ and $a \in \Sigma$.
Using the induction hypothesis, we obtain
\[
\widehat{\delta'}(q'_0, wa) = \delta'(\widehat{\delta'}(q'_0, w), a) = \delta'(\widehat{\delta}(q_0, w), a)
= \overline{\delta(\widehat{\delta}(q_0, w), a)} = \widehat{\delta}(q_0, wa).
\]

Now, by definition we have
\begin{gather*}
w \in L(M) \Leftrightarrow \widehat{\delta}(q_0, w) \cap F \ne \emptyset,\\
w \in L(M') \Leftrightarrow \widehat{\delta'}(q'_0, w) \in F' \Leftrightarrow \widehat{\delta'}(q'_0, w) \cap F \ne \emptyset,
\end{gather*}
which implies $L(M) = L(M')$ due to \eqref{eqn:DeltaD=DeltaE}.
\end{proof}
