\input{preamble.tex}
\begin{document}
\setcounter{section}{2}
\setcounter{subsection}{2}
\setcounter{dfn}{3}

\begin{exl}
Let us prove the tautology $A \to A$.
First, substitute in the second axiom $(A \to A)$ for $B$ and $A$ for $C$:
\[
\vdash (A \to ((A \to A) \to A)) \to ((A \to (A \to A)) \to (A \to A))
\]
Now substitute $(A \to A)$ for $B$ in the first axiom:
\[
\vdash (A \to ((A \to A) \to A))
\]
This coincides with the ``left half'' of the previous formula, so by modus ponens we infer the ``right half'' of that formula:
\[
\vdash (A \to (A \to A)) \to (A \to A)
\]
Now take the first axiom with $B$ substituted for $A$:
\[
\vdash (A \to (A \to A)).
\]
This is the left half of the previous formula, so again by modus ponens we infer
\[
\vdash (A \to A),
\]
and the proof is finished.
\end{exl}

\end{document}
