\section{Own summary}


\subsection{Equivalences between propositional formulas}

There are several simple and useful equivalences between propositional formulas.
\begin{itemize}
\item
Associativity laws
\[
(A \wedge B) \wedge C \simeq A \wedge (B \wedge C) \qquad (A \vee B) \vee C \simeq A \vee (B \vee C)
\]
\item
Commutativity laws
\[
A \wedge B \simeq B \wedge A \qquad A \vee B \simeq B \vee A
\]
\item
Distributivity laws
\[
A \wedge (B \vee C) \simeq (A \wedge B) \vee (A \wedge C) \qquad A \vee (B \wedge C) \simeq (A \vee B) \wedge (A \vee C)
\]
\item
De Morgan's laws
\[
\neg(A \wedge B) \simeq \neg A \vee \neg B \qquad \neg(A \vee B) \simeq \neg A \wedge \neg B
\]
\item
Idempotency laws
\[
A \wedge A \simeq A \qquad A \vee A \simeq A
\]
\item
Double negation law
\[
\neg\neg A \simeq A
\]
\end{itemize}

The associativity laws allow us to omit parentheses in conjunctions or disjunctions.
Due to it we can allow abuse of notation and write strings like this one:
\[
p \wedge q \wedge r \wedge s.
\]
This is against the syntax rules.
In order to conform the rules, we must put some parentheses.
This leads to several different propositional formulas, like $((p \wedge q) \wedge (r \wedge s))$ or $((p \wedge (q \wedge r)) \wedge s)$.
Although these formulas are different, they are logically equivalent.
Thus, the string $p \wedge q \wedge r \wedge s$ stands for a class of equivalent formulas.

The distributivity laws allow us to operate with brackets as if $\wedge$ is the multiplication and $\vee$ is the addition
or vice versa.
For example,
\[
\neg p \vee (p \wedge q) \simeq (\neg p \vee p) \wedge (\neg p \vee q).
\]

Let us extend the language $\Prop$ by adding two new symbols $\top$ and $\perp$.
We define a language $\widetilde{\Prop}$ by adding to the point 1. in Definition \ref{dfn:PropForm} that $\top$ and $\perp$ belong to $\widetilde{\Prop}$
and leaving the other conditions as they are.
The symbols $\top$ and $\perp$ are \emph{logical constants}: when computing the truth value of a proposition $A$
we replace each $\top$ by $1$ and each $\perp$ by $0$.
In $\widetilde{\Prop}$ there are the following logical equivalences.
\begin{itemize}
\item
Laws of zero and one.
\begin{gather*}
(A \wedge \perp) \simeq \perp \qquad (A \vee \perp) \simeq A\\
(A \wedge \top) \simeq A \qquad (A \vee \top) \simeq \top\\
(A \wedge \neg A) \simeq \perp \qquad (A \vee \neg A) \simeq \top
\end{gather*}
\end{itemize}


\subsection{All inference rules}

\begin{align*}
&(\wedge\text{ \rm left}):\
\AxiomC{$A, B, \Gamma \vdash \Delta$}
\UnaryInfC{$A \wedge B, \Gamma \vdash \Delta$}
\DisplayProof
&&(\wedge\text{ \rm right}):\
\AxiomC{$\Gamma \vdash A, \Delta$}
\AxiomC{$\Gamma \vdash B, \Delta$}
\BinaryInfC{$\Gamma \vdash A \wedge B, \Delta$}
\DisplayProof
\\
&(\vee\text{ \rm left}):\
\AxiomC{$A, \Gamma \vdash \Delta$}
\AxiomC{$B, \Gamma \vdash \Delta$}
\BinaryInfC{$A \vee B, \Gamma \vdash \Delta$}
\DisplayProof
&&(\vee\text{ \rm right}):\
\AxiomC{$\Gamma \vdash A, B, \Delta$}
\UnaryInfC{$\Gamma \vdash A \vee B, \Delta$}
\DisplayProof
\\
&(\to\text{ \rm left}):\
\AxiomC{$\Gamma \vdash A, \Delta$}
\AxiomC{$\Gamma, B \vdash \Delta$}
\BinaryInfC{$A \to B, \Gamma \vdash \Delta$}
\DisplayProof
&&(\to\text{ \rm right}):\
\AxiomC{$\Gamma, A \vdash B, \Delta$}
\UnaryInfC{$\Gamma \vdash A \to B, \Delta$}
\DisplayProof
\\
&(\neg\text{ \rm left}):\
\AxiomC{$\Gamma \vdash A, \Delta$}
\UnaryInfC{$\neg A, \Gamma \vdash \Delta$}
\DisplayProof
&&(\neg\text{ \rm right}):\
\AxiomC{$A, \Gamma \vdash \Delta$}
\UnaryInfC{$\Gamma \vdash \neg A, \Delta$}
\DisplayProof
\end{align*}

Own comment:
\begin{itemize}
  \item \textbf{$A[t/x]$} \textit{replace $x$ with a term (reuse term or add a new one)}
  \item \textbf{$A[y/x]$} \textit{replace $x$ with a new free variable}
\end{itemize}

\begin{align*}
&(\forall\text{ \rm left}):\
\AxiomC{$A[t/x], \forall x A, \Gamma \vdash \Delta$}
\UnaryInfC{$\forall x A, \Gamma \vdash \Delta$}
\DisplayProof
&&(\forall\text{ \rm right}):\
\AxiomC{$\Gamma \vdash A[y/x], \Delta$}
\UnaryInfC{$\Gamma \vdash \forall x A, \Delta$}
\DisplayProof
\\
&(\exists\text{ \rm left}):\
\AxiomC{$A[y/x], \Gamma \vdash \Delta$}
\UnaryInfC{$\exists x A, \Gamma \vdash \Delta$}
\DisplayProof
&&(\exists\text{ \rm right}):\
\AxiomC{$\Gamma \vdash A[t/x], \exists x A, \Delta$}
\UnaryInfC{$\Gamma \vdash \exists x A, \Delta$}
\DisplayProof
\end{align*}


