\input{preamble.tex}
\begin{document}
\setcounter{section}{2}
\setcounter{subsection}{2}
\setcounter{dfn}{6}

\begin{exl}
Let us prove the formula $\exists x(P \to Q(x)) \to (P \to \exists y Q(y))$.
\begin{prooftree}
\AxiomC{$P \vdash P, \exists y Q(y)$}
\AxiomC{$Q(z_1), P \vdash Q(z_1), \exists y Q(y)$}
\UnaryInfC{$Q(z_1), P \vdash \exists y Q(y)$}
\BinaryInfC{$P, P \to Q(z_1) \vdash \exists y Q(y)$}
\UnaryInfC{$P \to Q(z_1) \vdash P \to \exists y Q(y)$}
\UnaryInfC{$\exists x(P \to Q(x)) \vdash P \to \exists y Q(y)$}
\UnaryInfC{$\vdash \exists x(P \to Q(x)) \to (P \to \exists y Q(y))$}
\end{prooftree}

At the second step we are introducing a new variable $z_1$ while applying the left $\exists$ inference rule.
After application of the branching left $\to$ rule we obtain an axiom on the left (with $P$ on both sides of $\vdash$).
On the right we are applying the right $\exists$ rule, where we can make a clever choice of a term to substitute for $y$.
Choosing $z_1/y$ as the substitution, we obtain two equal terms on both sides of $\vdash$, and the proof tree is finished.
\end{exl}

\end{document}
