\input{preamble.tex}
\begin{document}
\setcounter{section}{3}
\setcounter{subsection}{5}
\setcounter{dfn}{36}


\begin{proof}[Proof of Theorem \ref{thm:ConstUndecid}]
Assume that $T$ is decidable.
Consider the set
\[
X = \{(m,n) \mid m = \sharp A(\cdot), T \vdash A[\underline{n}/\cdot]\} \subset \N^2.
\]
(Here $A(\cdot)$ means that $A$ has one free variable, and $A[t/\cdot]$ means substitution of term $t$ for this variable.)
Since $T$ is decidable, the set $X$ is recursive (there is an algorithm which decides whether $(m,n) \in X$ or not).

Now let
\[
Y = \{n \mid (n,n) \notin X\}.
\]
Clearly, since $X$ is recursive, so is $Y$.
By Theorem \ref{thm:ReprThm}, the set $Y$ is representable.
That is, there is a formula $B(y)$ such that
\begin{gather*}
n \in Y \Rightarrow PA_0 \vdash B[\underline{n}/y]\\
n \notin Y \Rightarrow PA_0 \vdash \neg B[\underline{n}/y]
\end{gather*}
Since $T \supset PA_0$, for every $C$ such that $PA_0 \vdash C$ we also have $T \vdash C$.

Now let $n = \sharp B(y)$.
Let us ask ourselves if $n \in Y$ or not. Assume $n \in Y$.
By definition of $Y$, $X$, and $n$ we have
\[
n \in Y \Rightarrow (n,n) \notin X \Rightarrow T \not\vdash B[\underline{n}/y] \Rightarrow T \vdash \neg B[\underline{n}/y].
\]
On the other hand, by definition of $B(y)$ we have
\[
n \in Y \Rightarrow T \vdash B[\underline{n}/y],
\]
which implies that $T$ is incoherent.
If we assume that $n \notin Y$, then we derive similarly that $T \vdash B[\underline{n}/y]$ and $T \vdash \neg B[\underline{n}/y]$.

Thus the decidability assumption contradicts the consistency assumption, and the theorem is proved.
\end{proof}



\end{document}
