\input{preamble.tex}
\begin{document}
\setcounter{section}{3}
\setcounter{subsection}{2}
\setcounter{dfn}{23}

% \begin{proof}
% If $T \vdash A$, then $T \cup \{\neg A\} \vdash A$ and $T \cup \{\neg A\} \vdash \neg A$.
% Thus $T \cup \{\neg A\}$ is not consistent.
% 
% In the opposite direction, if $T \cup \{\neg A\}$ is not consistent, then we have
% \[
% T \cup \{\neg A\} \vdash B, \neg B \vdash A
% \]
% (because $(B \wedge \neg B) \to A$ is a tautology).
% By Lemma \ref{lem:DedThm}, $T \cup \{\neg A\} \vdash A$ implies $T \vdash (\neg A \to A)$.
% Since $(\neg A \to A) \to A$ is a tautology, we get $T \vdash A$.
% \end{proof}
% 
% \begin{proof}[Proof of equivalence Theorem \ref{thm:Complete1} $\Leftrightarrow$ \ref{thm:Complete2}]
% If $A$ is not a theorem of $T$, then $T \cup \{\neg A\}$ is consistent (Lemma \ref{lem:ThmNotConsist}), thus satisfiable (Lemma \ref{lem:SatConsist}).
% Thus there is a model for $T$ in which $A$ is false.
% \end{proof}




\end{document}
