\input{preamble.tex}
\begin{document}
\setcounter{section}{2}
\setcounter{subsection}{2}
\setcounter{dfn}{6}

(Note that it is also well-defined for any value of $b_0$ provided that $A(x)$ is a polynomial, but we are not going to need this.)

The composition is compatible with sum and product:
\begin{gather*}
\text{if } C(x) = A(x) + B(x), \text{ then } C(D(x)) = A(D(x)) + B(D(x)),\\
\text{if } C(x) = A(x)B(x), \text{ then } C(D(x)) = A(D(x))B(D(x)).
\end{gather*}

This implies in particular that for every formal power series $B(x)$ with $b_0 = 0$ one has
\[
(1 - B(x))^{-1} = 1 + B(x) + (B(x))^2 + \cdots.
\]


\end{document}
