\subsection{Sum rule}
\begin{center}
\emph{If $X \cap Y = \emptyset$, then $|X \cup Y| = |X| + |Y|$.}
\end{center}

More generally,
\begin{center}
\parbox{.9\textwidth}{\emph{If the sets $X_1, \ldots, X_n$ are pairwise disjoint
(that is $X_i \cap X_j = \emptyset$ for all $i \ne j$),
then $|X_1 \cup X_2 \cup \cdots \cup X_n| = |X_1| + |X_2| + \cdots + |X_n|$.}}
\end{center}
Formally, this follows by induction on $n$ from the sum rule for two sets.

Later we will learn how to proceed if the sets are not disjoint.
