The composition is not always well-defined. Indeed, we have
\[
A(B(x)) = a_0 + a_1(b_0 + b_1 x + b_2 x^2 + \cdots) + a_2(b_0 + b_1 x + b_2 x^2 + \cdots)^2 + \cdots.
\]
In particular, the constant term is an infinite sum $a_0 + a_1 b_0 + a_2 b_0^2 + \cdots$, which is not good.
However, if $b_0 = 0$, then we have
\[
a_k (B(x))^k = a_k (b_1 x + b_2 x^2 + \cdots)^k = a_k b_1^k x^k + \text{ higher order terms},
\]
so that the coefficient at $x^k$ in $A(B(x))$ is a finite expression in $a_i, b_j$.
Thus we arrive to the following conclusion.
