\input{../preamble.tex}
\begin{document}
\setcounter{section}{3}
\setcounter{subsection}{3}
\setcounter{dfn}{2}

\begin{proof}
One has
\[
\frac{1}{(1-x)^k} = \underbrace{(1+x+x^2+\cdots)\cdots(1+x+x^2+\cdots)}_{k}
\]
When one expands the brackets in the product on the right hand side,
one picks from the first brackets a monomial $x^{m_1}$, from the second $x^{m_2}$ and so on up to $x^{m_k}$ from the last brackets.
The product of these monomials is $x^{m_1+\cdots+m_k}$.
When one collects the monomials of degree $n$, one obtains a term $a_n x^n$,
where $n$ is the number of solutions of the equation
\[
m_1 + \cdots + m_k = n,
\]
where the unknowns $m_1, \ldots, m_k$ can take only non-negative integer values.
The number of solutions is exactly the number of weak compositions of $n$ from $k$ parts.
\end{proof}

Now, by applying the generalized binomial theorem one obtains
\[
\sum_{n=0}^\infty a_n x^n = \frac{1}{(1-x)^k} = (1-x)^{-k} = \sum_{n=0}^\infty (-1)^n \binom{-k}{n} x^n
\]
Thus we have
\[
a_n = (-1)^n \binom{-k}{n} = \binom{n+k-1}{n} = \binom{n+k-1}{k-1}.
\]




\end{document}